Linglib.lean
@@ -1151,7 +1151,6 @@ import Linglib.Phonology.OCP
 import Linglib.Phonology.OptimalityTheory.Antimatroid
 import Linglib.Phonology.OptimalityTheory.Cophonology
 import Linglib.Phonology.OptimalityTheory.Correspondence
-import Linglib.Phonology.OptimalityTheory.Doubling
 import Linglib.Phonology.OptimalityTheory.ElementaryRankingCondition
 import Linglib.Phonology.OptimalityTheory.Grammar
 import Linglib.Phonology.OptimalityTheory.HarmonicSerialism
